checkpoint of validating functions that return pointers. Defined:   1) An abstract call      call void fn (ret_tmp, ...)      %3 = getelementptr { i32*, i8*, i8* }* %ret_tmp, i32 0, i32 0      %4 = load i32** %3      %_base3 = getelementptr { i32*, i8*, i8* }* %ret_tmp, i32 0, i32 1      %call_repl_base = load i8** %_base3      %_bound4 = getelementptr { i32*, i8*, i8* }* %ret_tmp, i32 0, i32 2      %call_repl_bound = load i8** %_bound4
  2) An abstract ret
     %.ptr = getelementptr { i32*, i8*, i8* }* %shadow_ret, i32 0, %i32 0
     %.base = getelementptr { i32*, i8*, i8* }* %shadow_ret, i32 0, %i32 1
     store i8* %bitcast, i8** %.base
     %.bound = getelementptr { i32*, i8*, i8* }* %shadow_ret, i32 0, %i32 2
     store i8* %bitcast4, i8** %.bound
     store i32* %8, i32** %.ptr
     ret void
and consider these instructions as a single evaluation step.

Another interesting thing is function names can be variables, so we
cannot statically know which function a variable means.

  --This line, and those below, will be ignored--
M    vol/src/Extraction/extraction.v
M    vol/src/Extraction/symexe_aux.ml
M    vol/src/myocamlbuild.ml
M    vol/src/TV/sub_tv.v
M    vol/src/TV/sub_tv_correct.v
M    vol/src/Parser/tvcases/log
A    vol/src/Parser/tvcases/olden-ccured/bisort/renaming.db
A    vol/src/Parser/tvcases/olden-ccured/mst/renaming.db
A    vol/src/Parser/tvcases/olden-ccured/health/renaming.db
A    vol/src/Parser/tvcases/olden-ccured/tsp/renaming.db
A    vol/src/Parser/tvcases/olden-ccured/treeadd/renaming.db
A    vol/src/Parser/tvcases/olden-ccured/em3d/renaming.db
A    vol/src/Parser/tvcases/olden-ccured/bh/renaming.db
A    vol/src/Parser/tvcases/olden-ccured/power/renaming.db
A    vol/src/Parser/tvcases/olden-ccured/perimeter/renaming.db
M    vol/src/Parser/tvcases/milli/funcret/metadata.db
M    vol/src/Parser/tvcases/milli/funcret/renaming.db
M    vol/src/Parser/tvcases/test.sh
M    vol/src/Parser/tvcases/Makefile
M    vol/src/Parser/main.ml
M    vol/src/Parser/_tags
M    vol/src/Makefile
M    vol/src/_tags
M    vol/src/.metadata/.plugins/org.eclipse.core.runtime/.settings/org.eclipse.ui.prefs
M    vol/src/.metadata/.plugins/org.eclipse.ui.ide/dialog_settings.xml
M    vol/src/.metadata/.plugins/org.eclipse.ui.workbench/workbench.xml
M    vol/src/.metadata/.plugins/org.eclipse.core.resources/.safetable/org.eclipse.core.resources
M    vol/src/.metadata/.log


git-svn-id: https://webdav.seas.upenn.edu/svn/sol/vol@2829 eef5ea85-cc2e-0410-bd84-0fae1f012da8

src/Parser/main.ml
@@ -43,7 +43,7 @@ let main in_filename out_filename =
   let addr = Sub_tv.addrofbe_from_module coqom in
   metadata_to_file md addr "metadata.db";
   eprintf "SubTV=%b MTV=%b\n" (Sub_tv.tv_module coqim coqom) 
-          (Sub_tv.mtv_module coqom);
+          (Sub_tv.mtv_module coqim coqom);
   
   (* Coq2llvm.translate_module coqom; *)
   
