src/myocamlbuild.ml
@@ -16,7 +16,10 @@ ocaml_lib ~extern:true "coq2llvm";;
 ocaml_lib ~extern:true "coq_pretty_printer";;
 ocaml_lib ~extern:true "globalstates";;
 ocaml_lib ~extern:true "eq_tv";;
+ocaml_lib ~extern:true "str";; 
+(* adding str before sub_tv is important, because sub_tv needs str, and
+ * ocamlbuild links libs in term of the order in the file. *)
 ocaml_lib ~extern:true "sub_tv";;
 
 flag ["link"; "ocaml"; "g++"] (S[A"-cc"; A"g++"]);;
-dep ["link"; "ocaml"; "use_bindings"; "using_sub_tv"; "using_eq_tv"] ;;
+dep ["link"; "ocaml"; "use_bindings"] ;;
