src/TV/sub_tv.v
@@ -69,6 +69,16 @@ Axiom INT_is_one : INT -> bool.
 *)
 Axiom rename_fid : id -> id.
 
+(* From a name in an output program to its original name in the input program. *)
+Axiom rename_fid_inv : id -> option id.
+
+Axiom rename_fid_prop1 : forall fid,
+  rename_fid_inv (rename_fid fid) = Some fid.
+
+Axiom rename_fid_prop2 : forall fid1 fid2,
+  rename_fid_inv fid1 = Some fid2 ->
+  rename_fid fid2 = fid1.
+
 (* In function f1, i1 is renamed to be (rename_id f1 i1) *)
 Axiom rename_id : id -> id -> id.
 
@@ -105,6 +115,203 @@ end.
 
 Definition eq_sterm_upto_cast (st1 st2:sterm) : bool :=
 eq_sterm (remove_cast st1) (remove_cast st2).
+
+(***************************************************************)
+(** LLVM.syntax -> Symexe.syntax 
+ * 
+   If a function returns a pointer, e.g.
+     define i32* @test(i32 %mm) nounwind
+   Softbound translates it to be
+     define void @softbound_test({ i32*, i8*, i8* }* %shadow_ret, i32 %mm)
+
+   %shadow_ret is a returned pointer with its base and bound.
+
+   At callsite,
+     %3 = tail call i32* @test(i32 %2) nounwind
+   is translated to be
+
+     call void @softbound_test({ i32*, i8*, i8* }* %ret_tmp, i32 %2)
+     %3 = getelementptr { i32*, i8*, i8* }* %ret_tmp, i32 0, i32 0
+     %4 = load i32** %3          
+     %_base3 = getelementptr { i32*, i8*, i8* }* %ret_tmp, i32 0, i32 1
+     %call_repl_base = load i8** %_base3       
+     %_bound4 = getelementptr { i32*, i8*, i8* }* %ret_tmp, i32 0, i32 2
+     %call_repl_bound = load i8** %_bound4   
+
+   The idea is defining an abstract call
+     {%3, %call_repl_base, %call_repl_bound} = 
+       call void @softbound_test({ i32*, i8*, i8* }* %ret_tmp, i32 %2)
+   that equals to the above seven instructions.
+
+*)
+
+Inductive icall : Set :=
+ | icall_nptr : id -> noret -> tailc -> typ -> value -> params -> icall
+ | icall_ptr : id -> id -> id -> typ -> value -> id -> params -> icall.
+
+Record isubblock := mkiSB
+{
+  iNBs : list nbranch;
+  icall_cmd : icall
+}.
+
+Lemma isCall_inv : forall (c:cmd), isCall c = true -> 
+  id * noret * tailc * typ * value * params.
+Proof.
+  destruct c; intros H; try solve [inversion H].
+  split; auto.
+Defined. 
+
+(*
+     %3 = getelementptr { i32*, i8*, i8* }* %ret_tmp, i32 0, i32 0
+     %4 = load i32** %3          
+     %_base3 = getelementptr { i32*, i8*, i8* }* %ret_tmp, i32 0, i32 1
+     %call_repl_base = load i8** %_base3       
+     %_bound4 = getelementptr { i32*, i8*, i8* }* %ret_tmp, i32 0, i32 2
+     %call_repl_bound = load i8** %_bound4    
+*)
+Definition gen_icall (v:value) (pa0:params) (c1 c2 c3 c4 c5 c6:cmd) 
+  : option icall :=
+match c1 with
+|insn_gep id11 _ t1 (value_id id12)
+   (Cons_list_value (value_const (const_int _ i11 as c11)) 
+     (Cons_list_value (value_const (const_int _ i12 as c12)) 
+      Nil_list_value)) =>
+  match c2 with
+  |insn_load id21 t2 (value_id id22) _ =>
+    match c3 with 
+    |insn_gep id31 _ t3 (value_id id32) 
+       (Cons_list_value (value_const (const_int _ i31 as c31)) 
+         (Cons_list_value (value_const (const_int _ i32 as c32)) 
+         Nil_list_value)) =>
+      match c4 with
+      |insn_load id41 t4 (value_id id42) _ =>
+        match c5 with
+        |insn_gep id51 _ t5 (value_id id52)
+           (Cons_list_value (value_const (const_int _ i51 as c51)) 
+           (Cons_list_value (value_const (const_int _ i52 as c52)) 
+              Nil_list_value)) =>
+           match c6 with
+           |insn_load id61 t6 (value_id id62) _ =>
+              match pa0 with
+              | (
+                 typ_pointer t0,
+(*
+                 typ_pointer (typ_struct 
+                  (Cons_list_typ (typ_pointer _ as t01) 
+                  (Cons_list_typ (typ_pointer _ as t02)
+                  (Cons_list_typ (typ_pointer _ as t03) Nil_list_typ))) as t0),
+*)
+                 value_id id0)::pa0' =>
+                if (tv_typ t1 t3 && tv_typ t3 t5 && tv_typ t5 t0 &&
+(*
+                    tv_typ t2 t01 && tv_typ t4 t02 && tv_typ t6 t03 &&
+                    tv_typ t02 t03 && 
+*)
+                    eq_id id0 id12 && eq_id id0 id32 && eq_id id0 id52 &&
+                    eq_id id11 id22 && eq_id id31 id42 && eq_id id51 id62 &&
+                    eq_const c11 c12 && eq_const c11 c31 && eq_const c11 c51
+                   ) 
+                then 
+                  Some (icall_ptr id21 id41 id61 t2 v id0 pa0')
+                else None
+              | _ => None
+              end
+           | _ => None
+           end
+        | _ => None
+        end
+      | _ => None
+      end
+    | _ => None
+    end
+  | _ => None
+  end
+| _ => None
+end.
+
+(* e.g. calloc -> softbound_calloc *)
+Axiom syscall_returns_pointer : id -> bool.
+
+(* Ps is from the input program. *)
+Definition function_returns_pointer Ps1 fid2 : bool :=
+match (rename_fid_inv fid2) with
+| Some fid1 =>
+    match lookupFdefViaIDFromProducts Ps1 fid1 with      
+    | Some (fdef_intro (fheader_intro (typ_pointer _ as tp) _ _) _) => true
+    | _ => syscall_returns_pointer fid1
+    end
+| None => false
+end.
+
+Fixpoint cmds2isbs (Ps1:products) (cs:cmds) : (list isubblock*list nbranch) :=
+match cs with
+| nil => (nil,nil)
+| c::cs' =>
+  match (isCall_dec c) with
+  | left isnotcall => 
+    match (cmds2isbs Ps1 cs') with
+    | (nil, nbs0) => (nil, mkNB c isnotcall::nbs0) 
+    | (mkiSB nbs call0::sbs', nbs0) => 
+      (mkiSB (mkNB c isnotcall::nbs) call0::sbs', nbs0) 
+    end
+  | right iscall => 
+    let '(id1, nr1, tc1, t1, v1, pa1) := isCall_inv c iscall in
+    let '(sbs, nbs0, ic) :=
+(*
+    Do not check if the called function returns ptr. The problem is
+    v1 can be a value that represents a function pointer. Statically, we 
+    need more work to identidy it.
+
+    We check this property at tv_call.
+
+    match v1 with
+    | value_const (const_gid _ fid2) => 
+      if (function_returns_pointer Ps1 fid2) then
+*)
+        match cs' with
+        | c1::c2::c3::c4::c5::c6::cs'' =>
+          match (gen_icall v1 pa1 c1 c2 c3 c4 c5 c6) with
+          | Some ic => (cmds2isbs Ps1 cs'', ic)
+          | None => (cmds2isbs Ps1 cs', icall_nptr id1 nr1 tc1 t1 v1 pa1)
+          end
+        | _ => (cmds2isbs Ps1 cs', icall_nptr id1 nr1 tc1 t1 v1 pa1)
+        end
+(* 
+      else (cmds2isbs Ps1 cs', icall_nptr id1 nr1 tc1 t1 v1 pa1)
+    | _ => (cmds2isbs Ps1 cs', icall_nptr id1 nr1 tc1 t1 v1 pa1)
+    end 
+*)
+    in (mkiSB nil ic::sbs, nbs0) 
+  end
+end.
+
+Inductive wf_inbranchs : list nbranch -> Prop :=
+| wf_inbranchs_intro : forall Ps cs nbs, 
+  cmds2isbs Ps cs = (nil, nbs) ->
+  NoDup (getCmdsIDs cs) ->
+  wf_inbranchs nbs.
+
+Inductive wf_isubblock : isubblock -> Prop :=
+| wf_isubblock_intro : forall nbs call0, 
+  wf_inbranchs nbs ->
+  wf_isubblock (mkiSB nbs call0).
+
+Inductive wf_isubblocks : list isubblock -> Prop :=
+| wf_isubblocks_nil : wf_isubblocks nil
+| wf_isubblocks_cons : forall sb sbs,
+  wf_isubblock sb ->
+  wf_isubblocks sbs ->
+  wf_isubblocks (sb::sbs).
+
+Inductive wf_iblock : block -> Prop :=
+| wf_iblock_intro : forall Ps l ps cs sbs nbs tmn, 
+  cmds2isbs Ps cs = (sbs,nbs) ->
+  wf_isubblocks sbs ->
+  wf_inbranchs nbs ->
+  wf_iblock (block_intro l ps cs tmn).
+
+Hint Constructors wf_isubblocks.
 
 (************************************************************)
 (* Generating metadata *) 
@@ -532,8 +739,6 @@ declare weak void @__hashLoadBaseBound(
 We assume 
   1) We have already checked that %addr_of_base, %addr_of_bound and %ptr_safe 
      are valid when being passed into @__hashLoadBaseBound. 
-    FIXME: Checking if they equal to "alloca..." 
-
   2) __hashLoadBaseBound does not change %base, %bound and %ptr_safe.
 
 So, %base, %bound and %ptr_safe are safe to load w/o memsafety checks.
@@ -574,176 +779,6 @@ Axiom tv_id_injective1 : forall fid id1 id2 id1' id2',
 Axiom tv_id_injective2 : forall fid id1 id2 id1' id2',
   id1 <> id2 -> tv_id fid id1 id1' -> tv_id fid id2 id2' -> id1' <> id2'.
 
-Definition tv_value fid v1 v2 : bool :=
-match (v1, v2) with
-| (value_id id1, value_id id2) => tv_id fid id1 id2
-| (v1, v2) => eq_value v1 v2
-end.
-
-Fixpoint tv_sterm fid (st st':sterm) : bool :=
-match (st, st') with
-| (sterm_val v, sterm_val v') => tv_value fid v v'
-| (sterm_bop b sz st1 st2, sterm_bop b' sz' st1' st2') =>
-    sumbool2bool _ _ (bop_dec b b') && sumbool2bool _ _ (Size.dec sz sz') &&
-    tv_sterm fid st1 st1' && tv_sterm fid st2 st2'
-| (sterm_fbop b f st1 st2, sterm_fbop b' f' st1' st2') =>
-    sumbool2bool _ _ (fbop_dec b b') && 
-    sumbool2bool _ _ (floating_point_dec f f') &&
-    tv_sterm fid st1 st1' && tv_sterm fid st2 st2'
-| (sterm_extractvalue t st1 cs, sterm_extractvalue t' st1' cs') =>
-    tv_typ t t' && tv_sterm fid st1 st1' &&
-  sumbool2bool _ _ (list_const_dec cs cs')
-| (sterm_insertvalue t1 st1 t2 st2 cs, 
-   sterm_insertvalue t1' st1' t2' st2' cs') =>
-    tv_typ t1 t1' && tv_sterm fid st1 st1' && 
-    tv_typ t2 t2' && tv_sterm fid st2 st2' &&
-    sumbool2bool _ _ (list_const_dec cs cs')
-| (sterm_malloc sm t st1 a, sterm_malloc sm' t' st1' a') =>
-    tv_smem fid sm sm' && tv_typ t t' && tv_sterm fid st1 st1' && tv_align a a'
-| (sterm_alloca sm t st1 a, sterm_alloca sm' t' st1' a') =>
-    tv_smem fid sm sm' && tv_typ t t' && tv_sterm fid st1 st1' && tv_align a a'
-| (sterm_load sm t st1 a, sterm_load sm' t' st1' a') =>
-    tv_smem fid sm sm' && tv_typ t t' && tv_sterm fid st1 st1' && tv_align a a'
-| (sterm_gep i t st1 sts2, sterm_gep i' t' st1' sts2') =>
-    sumbool2bool _ _ (bool_dec i i') && tv_typ t t' &&
-    tv_sterm fid st1 st1' && tv_list_sterm fid sts2 sts2'
-| (sterm_trunc top t1 st1 t2, sterm_trunc top' t1' st1' t2') =>
-    sumbool2bool _ _ (truncop_dec top top') && tv_typ t1 t1' &&
-    tv_sterm fid st1 st1' && tv_typ t2 t2'
-| (sterm_ext eo t1 st1 t2, sterm_ext eo' t1' st1' t2') =>
-    sumbool2bool _ _ (extop_dec eo eo') && tv_typ t1 t1' &&
-    tv_sterm fid st1 st1' && tv_typ t2 t2' 
-| (sterm_cast co t1 st1 t2, sterm_cast co' t1' st1' t2') =>
-    sumbool2bool _ _ (castop_dec co co') && tv_typ t1 t1' &&
-    tv_sterm fid st1 st1' && tv_typ t2 t2' 
-| (sterm_icmp c t st1 st2, sterm_icmp c' t' st1' st2') =>
-    sumbool2bool _ _ (cond_dec c c') && tv_typ t t' &&
-    tv_sterm fid st1 st1' && tv_sterm fid st2 st2'
-| (sterm_fcmp c ft st1 st2, sterm_fcmp c' ft' st1' st2') =>
-    sumbool2bool _ _ (fcond_dec c c') &&
-    sumbool2bool _ _ (floating_point_dec ft ft') &&
-    tv_sterm fid st1 st1' && tv_sterm fid st2 st2'
-| (sterm_phi t stls, sterm_phi t' stls') =>
-    tv_typ t t' && tv_list_sterm_l fid stls stls'
-| (sterm_select st1 t st2 st3, sterm_select st1' t' st2' st3') =>
-    tv_sterm fid st1 st1' && tv_typ t t' && 
-    tv_sterm fid st2 st2' && tv_sterm fid st3 st3'
-| (sterm_lib sm i sts, sterm_lib sm' i' sts') =>
-    tv_smem fid sm sm' && eq_id i i' && tv_list_sterm fid sts sts'
-| _ => false
-end
-with tv_list_sterm fid (sts sts':list_sterm) : bool :=
-match (sts, sts') with
-| (Nil_list_sterm, Nil_list_sterm) => true
-| (Cons_list_sterm st sts0, Cons_list_sterm st' sts0') =>
-    tv_sterm fid st st' && tv_list_sterm fid sts0 sts0'
-| _ => false
-end
-with tv_list_sterm_l fid (stls stls':list_sterm_l) : bool :=
-match (stls, stls') with
-| (Nil_list_sterm_l, Nil_list_sterm_l) => true
-| (Cons_list_sterm_l st l stls0, Cons_list_sterm_l st' l' stls0') =>
-    tv_sterm fid st st' && sumbool2bool _ _ (l_dec l l') && 
-    tv_list_sterm_l fid stls0 stls0'
-| _ => false
-end
-with tv_smem fid (sm1 sm2:smem) : bool :=
-match (sm1, sm2) with
-| (smem_init, _) => true
-| (smem_malloc sm1 t1 st1 a1, smem_malloc sm2 t2 st2 a2) =>
-    tv_smem fid sm1 sm2 && tv_typ t1 t2 && tv_sterm fid st1 st2 && tv_align a1 a2
-| (smem_alloca sm1 t1 st1 a1, smem_alloca sm2 t2 st2 a2) =>
-    if (tv_typ t1 t2 && tv_sterm fid st1 st2 && tv_align a1 a2)
-    then tv_smem fid sm1 sm2
-    else tv_smem fid (smem_alloca sm1 t1 st1 a1) sm2
-| (smem_free sm1 t1 st1, smem_free sm2 t2 st2) =>
-    tv_smem fid sm1 sm2 && tv_typ t1 t2 && tv_sterm fid st1 st2
-| (smem_load sm1 t1 st1 a1, smem_load sm2 t2 st2 a2) =>
-    if (tv_typ t1 t2 && tv_sterm fid st1 st2 && tv_align a1 a2)
-    then tv_smem fid sm1 sm2
-    else tv_smem fid (smem_load sm1 t1 st1 a1) sm2
-| (smem_store sm1 t1 st11 st12 a1, smem_store sm2 t2 st21 st22 a2) =>
-    tv_smem fid sm1 sm2 && tv_typ t1 t2 && tv_sterm fid st11 st21 &&
-    tv_sterm fid st12 st22 && tv_align a1 a2
-| (smem_lib sm1 fid1 sts1, smem_lib sm2 fid2 sts2) => 
-    if (eq_id fid1 fid2 && tv_list_sterm fid sts1 sts2)
-    then tv_smem fid sm1 sm2
-    else tv_smem fid (smem_lib sm1 fid1 sts1) sm2
-| (sm1, smem_lib sm2 fid sts) => smem_lib_sub fid && tv_smem fid sm1 sm2
-| (sm1, smem_alloca sm2 t2 st2 a2) => tv_smem fid sm1 sm2
-| (sm1, smem_load sm2 t2 st2 a2) => 
-  (* We check load_from_metadata to ensure that the behavior of output programs 
-   * preserves input's. If we did not check, the additional load may be stuck. 
-   *)
-    tv_smem fid sm1 sm2 && load_from_metadata sm2 st2
-| _ => false
-end.
-
-Fixpoint tv_sframe fid (sf1 sf2:sframe) : bool :=
-match (sf1, sf2) with
-| (sframe_init, _) => true
-| (sframe_alloca sm1 sf1 t1 st1 a1, sframe_alloca sm2 sf2 t2 st2 a2) =>
-    if (tv_smem fid sm1 sm2 && tv_typ t1 t2 && 
-        tv_sterm fid st1 st2 && tv_align a1 a2)
-    then tv_sframe fid sf1 sf2
-    else tv_sframe fid (sframe_alloca sm1 sf1 t1 st1 a1) sf2
-| _ => false
-end.
-
-Fixpoint tv_smap fid (sm1 sm2:smap) : bool :=
-match sm1 with
-| nil => true
-| (id1,st1)::sm1' =>
-  match lookupAL _ sm2 (rename_id fid id1) with
-  | None => false
-  | Some st2 => tv_sterm fid st1 st2 && tv_smap fid sm1' sm2
-  end
-end.
-
-Definition sub_sstate fid s1 s2 := 
-  tv_smap fid s1.(STerms) s2.(STerms) = true /\ 
-  tv_smem fid s1.(SMem) s2.(SMem) = true /\
-  tv_sframe fid s1.(SFrame) s2.(SFrame) = true /\ s1.(SEffects) = s2.(SEffects).
-
-Lemma sstate_sub_dec : forall fid (sts1 sts2:sstate), 
-  uniq sts1.(STerms) -> {sub_sstate fid sts1 sts2} + {~sub_sstate fid sts1 sts2}.
-Proof.
-Ltac done_right' := 
-  right; intro J ; destruct J as [ J1 [J2 [J3 J4]]]; simpl in *; auto.
-
-  intros fid sts1 sts2 Huniq.
-  destruct sts1 as [st1 sm1 sf1 se1].
-  destruct sts2 as [st2 sm2 sf2 se2].
-  destruct (@sterms_dec se1 se2); subst; try solve [done_right'].
-  unfold sub_sstate. simpl.
-  destruct (tv_smap fid st1 st2); auto.
-  destruct (tv_smem fid sm1 sm2); auto.
-  destruct (tv_sframe fid sf1 sf2); auto.
-    right. intro J ; destruct J as [ J1 [J2 [J3 J4]]]. inversion J3.
-    right. intro J ; destruct J as [ J1 [J2 [J3 J4]]]. inversion J2.
-    right. intro J ; destruct J as [ J1 [J2 [J3 J4]]]. inversion J1.
-Qed.
-
-Definition tv_cmds fid (nbs1 nbs2 : list nbranch) :=
-sumbool2bool _ _ 
-  (sstate_sub_dec fid 
-    (se_cmds sstate_init nbs1) 
-    (se_cmds sstate_init nbs2) 
-    (se_cmds_init_uniq nbs1)).
-
-(* Here, we check which function to call conservatively. In practice, a v1
- * is a function pointer, we should look up the function name from the 
- * FunTable. Since the LLVM IR takes function names as function pointers,
- * if a program does not assign them to be other variables, they should
- * be the same. *)
-Fixpoint tv_params fid (tsts1 tsts2:list (typ*sterm)) : bool :=
-match (tsts1, tsts2) with
-| (nil, _) => true
-| ((t1,st1)::tsts1', (t2,st2)::tsts2') => 
-  tv_typ t1 t2 && tv_sterm fid st1 st2 && tv_params fid tsts1' tsts2'
-| _ => false
-end.
-
 Definition tv_fid (fid1 fid2:id) := 
   eq_id (rename_fid fid1) fid2.
 
@@ -753,36 +788,323 @@ Axiom tv_fid_injective1 : forall fid1 fid2 fid1' fid2',
 Axiom tv_fid_injective2 : forall fid1 fid2 fid1' fid2',
   fid1 <> fid2 -> tv_fid fid1 fid1' -> tv_fid fid2 fid2' -> fid1' <> fid2'.
 
+Fixpoint tv_const fid (c c':const) : bool :=
+match (c, c') with
+| (const_zeroinitializer t0, const_zeroinitializer t0') => tv_typ t0 t0'
+| (const_int _ _, const_int _ _) 
+| (const_floatpoint _ _, const_floatpoint _ _)
+| (const_undef _, const_undef _)
+| (const_null _, const_null _) => eq_const c c'
+| (const_arr t0 cs0, const_arr t0' cs0') => 
+    tv_typ t0 t0' && tv_list_const fid cs0 cs0'
+| (const_struct cs0, const_struct cs0') => tv_list_const fid cs0 cs0'
+| (const_gid _ id0, const_gid _ id0') => 
+    tv_fid id0 id0' || tv_id fid id0 id0'
+| (const_truncop to0 c0 t0, const_truncop to0' c0' t0') =>
+    sumbool2bool _ _ (truncop_dec to0 to0') && tv_const fid c0 c0' &&
+    tv_typ t0 t0'
+| (const_extop eo0 c0 t0, const_extop eo0' c0' t0') =>
+    sumbool2bool _ _ (extop_dec eo0 eo0') && tv_const fid c0 c0' &&
+    tv_typ t0 t0'
+| (const_castop co0 c0 t0, const_castop co0' c0' t0') =>
+    sumbool2bool _ _ (castop_dec co0 co0') && tv_const fid c0 c0' &&
+    tv_typ t0 t0'
+| (const_gep ib0 c0 cs0, const_gep ib0' c0' cs0') =>
+    sumbool2bool _ _ (inbounds_dec ib0 ib0') && tv_const fid c0 c0' &&
+    tv_list_const fid cs0 cs0' 
+| (const_select c0 c1 c2, const_select c0' c1' c2') =>
+    tv_const fid c0 c0' && tv_const fid c1 c1' && tv_const fid c2 c2'
+| (const_icmp cd0 c0 c1, const_icmp cd0' c0' c1') =>
+    sumbool2bool _ _ (cond_dec cd0 cd0') &&
+    tv_const fid c0 c0' && tv_const fid c1 c1'
+| (const_fcmp fd0 c0 c1, const_fcmp fd0' c0' c1') =>
+    sumbool2bool _ _ (fcond_dec fd0 fd0') &&
+    tv_const fid c0 c0' && tv_const fid c1 c1'
+| (const_extractvalue c0 cs0, const_extractvalue c0' cs0') =>
+    tv_const fid c0 c0' && tv_list_const fid cs0 cs0'
+| (const_insertvalue c0 c1 cs0, const_insertvalue c0' c1' cs0') =>
+    tv_const fid c0 c0' && tv_const fid c c1' && tv_list_const fid cs0 cs0'
+| (const_bop b0 c0 c1, const_bop b0' c0' c1') =>
+    sumbool2bool _ _ (bop_dec b0 b0') && 
+    tv_const fid c0 c0' && tv_const fid c1 c1'
+| (const_fbop f0 c0 c1, const_fbop f0' c0' c1') =>
+    sumbool2bool _ _ (fbop_dec f0 f0') && 
+    tv_const fid c0 c0' && tv_const fid c1 c1'
+| _ => false
+end
+with tv_list_const fid (cs cs':list_const) : bool :=
+match (cs, cs') with
+| (Nil_list_const, Nil_list_const) => true
+| (Cons_list_const c0 cs0, Cons_list_const c0' cs0') => 
+    tv_const fid c0 c0' && tv_list_const fid cs0 cs0'
+| _ => false
+end.
+
+Definition tv_value fid v1 v2 : bool :=
+match (v1, v2) with
+| (value_id id1, value_id id2) => tv_id fid id1 id2
+| (value_const c1, value_const c2) => tv_const fid c1 c2
+| _ => false
+end.
+
+Definition store_to_ret Ps1 Ps2 fid2 (ptr:sterm) : bool :=
+if (function_returns_pointer Ps1 fid2) then
+   match lookupFdefViaIDFromProducts Ps2 fid2 with      
+   | Some (fdef_intro (fheader_intro _  _ ((_,ret)::_)) _) =>
+       eq_sterm (get_ptr_object ptr) (sterm_val (value_id ret))
+   | _ => false
+   end
+else false.
+
+Fixpoint tv_sterm Ps1 Ps2 fid (st st':sterm) : bool :=
+match (st, st') with
+| (sterm_val v, sterm_val v') => tv_value fid v v'
+| (sterm_bop b sz st1 st2, sterm_bop b' sz' st1' st2') =>
+    sumbool2bool _ _ (bop_dec b b') && sumbool2bool _ _ (Size.dec sz sz') &&
+    tv_sterm Ps1 Ps2 fid st1 st1' && tv_sterm Ps1 Ps2 fid st2 st2'
+| (sterm_fbop b f st1 st2, sterm_fbop b' f' st1' st2') =>
+    sumbool2bool _ _ (fbop_dec b b') && 
+    sumbool2bool _ _ (floating_point_dec f f') &&
+    tv_sterm Ps1 Ps2 fid st1 st1' && tv_sterm Ps1 Ps2 fid st2 st2'
+| (sterm_extractvalue t st1 cs, sterm_extractvalue t' st1' cs') =>
+    tv_typ t t' && tv_sterm Ps1 Ps2 fid st1 st1' &&
+  sumbool2bool _ _ (list_const_dec cs cs')
+| (sterm_insertvalue t1 st1 t2 st2 cs, 
+   sterm_insertvalue t1' st1' t2' st2' cs') =>
+    tv_typ t1 t1' && tv_sterm Ps1 Ps2 fid st1 st1' && 
+    tv_typ t2 t2' && tv_sterm Ps1 Ps2 fid st2 st2' &&
+    sumbool2bool _ _ (list_const_dec cs cs')
+| (sterm_malloc sm t st1 a, sterm_malloc sm' t' st1' a') =>
+    tv_smem Ps1 Ps2 fid sm sm' && tv_typ t t' && 
+    tv_sterm Ps1 Ps2 fid st1 st1' && tv_align a a'
+| (sterm_alloca sm t st1 a, sterm_alloca sm' t' st1' a') =>
+    tv_smem Ps1 Ps2 fid sm sm' && tv_typ t t' && 
+    tv_sterm Ps1 Ps2 fid st1 st1' && tv_align a a'
+| (sterm_load sm t st1 a, sterm_load sm' t' st1' a') =>
+    tv_smem Ps1 Ps2 fid sm sm' && tv_typ t t' && 
+    tv_sterm Ps1 Ps2 fid st1 st1' && tv_align a a'
+| (sterm_gep i t st1 sts2, sterm_gep i' t' st1' sts2') =>
+    sumbool2bool _ _ (bool_dec i i') && tv_typ t t' &&
+    tv_sterm Ps1 Ps2 fid st1 st1' && tv_list_sterm Ps1 Ps2 fid sts2 sts2'
+| (sterm_trunc top t1 st1 t2, sterm_trunc top' t1' st1' t2') =>
+    sumbool2bool _ _ (truncop_dec top top') && tv_typ t1 t1' &&
+    tv_sterm Ps1 Ps2 fid st1 st1' && tv_typ t2 t2'
+| (sterm_ext eo t1 st1 t2, sterm_ext eo' t1' st1' t2') =>
+    sumbool2bool _ _ (extop_dec eo eo') && tv_typ t1 t1' &&
+    tv_sterm Ps1 Ps2 fid st1 st1' && tv_typ t2 t2' 
+| (sterm_cast co t1 st1 t2, sterm_cast co' t1' st1' t2') =>
+    sumbool2bool _ _ (castop_dec co co') && tv_typ t1 t1' &&
+    tv_sterm Ps1 Ps2 fid st1 st1' && tv_typ t2 t2' 
+| (sterm_icmp c t st1 st2, sterm_icmp c' t' st1' st2') =>
+    sumbool2bool _ _ (cond_dec c c') && tv_typ t t' &&
+    tv_sterm Ps1 Ps2 fid st1 st1' && tv_sterm Ps1 Ps2 fid st2 st2'
+| (sterm_fcmp c ft st1 st2, sterm_fcmp c' ft' st1' st2') =>
+    sumbool2bool _ _ (fcond_dec c c') &&
+    sumbool2bool _ _ (floating_point_dec ft ft') &&
+    tv_sterm Ps1 Ps2 fid st1 st1' && tv_sterm Ps1 Ps2 fid st2 st2'
+| (sterm_phi t stls, sterm_phi t' stls') =>
+    tv_typ t t' && tv_list_sterm_l Ps1 Ps2 fid stls stls'
+| (sterm_select st1 t st2 st3, sterm_select st1' t' st2' st3') =>
+    tv_sterm Ps1 Ps2 fid st1 st1' && tv_typ t t' && 
+    tv_sterm Ps1 Ps2 fid st2 st2' && tv_sterm Ps1 Ps2 fid st3 st3'
+| (sterm_lib sm i sts, sterm_lib sm' i' sts') =>
+    tv_smem Ps1 Ps2 fid sm sm' && eq_id i i' && 
+    tv_list_sterm Ps1 Ps2 fid sts sts'
+| _ => false
+end
+with tv_list_sterm Ps1 Ps2 fid (sts sts':list_sterm) : bool :=
+match (sts, sts') with
+| (Nil_list_sterm, Nil_list_sterm) => true
+| (Cons_list_sterm st sts0, Cons_list_sterm st' sts0') =>
+    tv_sterm Ps1 Ps2 fid st st' && tv_list_sterm Ps1 Ps2 fid sts0 sts0'
+| _ => false
+end
+with tv_list_sterm_l Ps1 Ps2 fid (stls stls':list_sterm_l) : bool :=
+match (stls, stls') with
+| (Nil_list_sterm_l, Nil_list_sterm_l) => true
+| (Cons_list_sterm_l st l stls0, Cons_list_sterm_l st' l' stls0') =>
+    tv_sterm Ps1 Ps2 fid st st' && sumbool2bool _ _ (l_dec l l') && 
+    tv_list_sterm_l Ps1 Ps2 fid stls0 stls0'
+| _ => false
+end
+with tv_smem Ps1 Ps2 fid (sm1 sm2:smem) : bool :=
+match (sm1, sm2) with
+| (smem_init, _) => true
+| (smem_malloc sm1 t1 st1 a1, smem_malloc sm2 t2 st2 a2) =>
+    tv_smem Ps1 Ps2 fid sm1 sm2 && tv_typ t1 t2 && 
+    tv_sterm Ps1 Ps2 fid st1 st2 && tv_align a1 a2
+| (smem_alloca sm1 t1 st1 a1, smem_alloca sm2 t2 st2 a2) =>
+    if (tv_typ t1 t2 && tv_sterm Ps1 Ps2 fid st1 st2 && tv_align a1 a2)
+    then tv_smem Ps1 Ps2 fid sm1 sm2
+    else tv_smem Ps1 Ps2 fid (smem_alloca sm1 t1 st1 a1) sm2
+| (smem_free sm1 t1 st1, smem_free sm2 t2 st2) =>
+    tv_smem Ps1 Ps2 fid sm1 sm2 && tv_typ t1 t2 && tv_sterm Ps1 Ps2 fid st1 st2
+| (smem_load sm1 t1 st1 a1, smem_load sm2 t2 st2 a2) =>
+    if (tv_typ t1 t2 && tv_sterm Ps1 Ps2 fid st1 st2 && tv_align a1 a2)
+    then tv_smem Ps1 Ps2 fid sm1 sm2
+    else tv_smem Ps1 Ps2 fid (smem_load sm1 t1 st1 a1) sm2 &&
+         load_from_metadata sm2 st2
+| (smem_store sm1 t1 st11 st12 a1, smem_store sm2 t2 st21 st22 a2) =>
+    if (tv_typ t1 t2 && tv_sterm Ps1 Ps2 fid st11 st21 &&
+        tv_sterm Ps1 Ps2 fid st12 st22 && tv_align a1 a2)
+    then tv_smem Ps1 Ps2 fid sm1 sm2
+    else tv_smem Ps1 Ps2 fid (smem_store sm1 t1 st11 st12 a1) sm2 &&
+         store_to_ret Ps1 Ps2 (rename_fid fid) st22
+| (smem_lib sm1 fid1 sts1, smem_lib sm2 fid2 sts2) => 
+    if (eq_id fid1 fid2 && tv_list_sterm Ps1 Ps2 fid sts1 sts2)
+    then tv_smem Ps1 Ps2 fid sm1 sm2
+    else tv_smem Ps1 Ps2 fid (smem_lib sm1 fid1 sts1) sm2
+| (sm1, smem_lib sm2 lid sts) => smem_lib_sub lid && tv_smem Ps1 Ps2 fid sm1 sm2
+| (sm1, smem_alloca sm2 t2 st2 a2) => tv_smem Ps1 Ps2 fid sm1 sm2
+| (sm1, smem_load sm2 t2 st2 a2) => 
+  (* We check load_from_metadata to ensure that the behavior of output programs 
+   * preserves input's. If we did not check, the additional load may be stuck. 
+   *)
+    tv_smem Ps1 Ps2 fid sm1 sm2 && load_from_metadata sm2 st2
+| (sm1, smem_store sm2 t2 st21 st22 a2) => 
+  (* We check that the additional stores must be to shadow_ret. *)
+    tv_smem Ps1 Ps2 fid sm1 sm2 && store_to_ret Ps1 Ps2 (rename_fid fid) st22
+| _ => false
+end.
+
+Fixpoint tv_sframe Ps1 Ps2 fid (sf1 sf2:sframe) : bool :=
+match (sf1, sf2) with
+| (sframe_init, _) => true
+| (sframe_alloca sm1 sf1 t1 st1 a1, sframe_alloca sm2 sf2 t2 st2 a2) =>
+    if (tv_smem Ps1 Ps2 fid sm1 sm2 && tv_typ t1 t2 && 
+        tv_sterm Ps1 Ps2 fid st1 st2 && tv_align a1 a2)
+    then tv_sframe Ps1 Ps2 fid sf1 sf2
+    else tv_sframe Ps1 Ps2 fid (sframe_alloca sm1 sf1 t1 st1 a1) sf2
+| _ => false
+end.
+
+Fixpoint tv_smap Ps1 Ps2 fid (sm1 sm2:smap) : bool :=
+match sm1 with
+| nil => true
+| (id1,st1)::sm1' =>
+  match lookupAL _ sm2 (rename_id fid id1) with
+  | None => false
+  | Some st2 => tv_sterm Ps1 Ps2 fid st1 st2 && tv_smap Ps1 Ps2 fid sm1' sm2
+  end
+end.
+
+Definition sub_sstate Ps1 Ps2 fid s1 s2 := 
+  tv_smap Ps1 Ps2 fid s1.(STerms) s2.(STerms) = true /\ 
+  tv_smem Ps1 Ps2 fid s1.(SMem) s2.(SMem) = true /\
+  tv_sframe Ps1 Ps2 fid s1.(SFrame) s2.(SFrame) = true /\ 
+  s1.(SEffects) = s2.(SEffects).
+
+Lemma sstate_sub_dec : forall Ps1 Ps2 fid (sts1 sts2:sstate), 
+  uniq sts1.(STerms) -> 
+  {sub_sstate Ps1 Ps2 fid sts1 sts2} + {~sub_sstate Ps1 Ps2 fid sts1 sts2}.
+Proof.
+Ltac done_right' := 
+  right; intro J ; destruct J as [ J1 [J2 [J3 J4]]]; simpl in *; auto.
+
+  intros Ps1 Ps2 fid sts1 sts2 Huniq.
+  destruct sts1 as [st1 sm1 sf1 se1].
+  destruct sts2 as [st2 sm2 sf2 se2].
+  destruct (@sterms_dec se1 se2); subst; try solve [done_right'].
+  unfold sub_sstate. simpl.
+  destruct (tv_smap Ps1 Ps2 fid st1 st2); auto.
+  destruct (tv_smem Ps1 Ps2 fid sm1 sm2); auto.
+  destruct (tv_sframe Ps1 Ps2 fid sf1 sf2); auto.
+    right. intro J ; destruct J as [ J1 [J2 [J3 J4]]]. inversion J3.
+    right. intro J ; destruct J as [ J1 [J2 [J3 J4]]]. inversion J2.
+    right. intro J ; destruct J as [ J1 [J2 [J3 J4]]]. inversion J1.
+Qed.
+
+Definition tv_cmds Ps1 Ps2 fid (nbs1 nbs2 : list nbranch) :=
+sumbool2bool _ _ 
+  (sstate_sub_dec Ps1 Ps2 fid 
+    (se_cmds sstate_init nbs1) 
+    (se_cmds sstate_init nbs2) 
+    (se_cmds_init_uniq nbs1)).
+
+(* Here, we check which function to call conservatively. In practice, a v1
+ * is a function pointer, we should look up the function name from the 
+ * FunTable. Since the LLVM IR takes function names as function pointers,
+ * if a program does not assign them to be other variables, they should
+ * be the same. *)
+Fixpoint tv_params Ps1 Ps2 fid (tsts1 tsts2:list (typ*sterm)) : bool :=
+match (tsts1, tsts2) with
+| (nil, _) => true
+| ((t1,st1)::tsts1', (t2,st2)::tsts2') => 
+  tv_typ t1 t2 && tv_sterm Ps1 Ps2 fid st1 st2 && 
+  tv_params Ps1 Ps2 fid tsts1' tsts2'
+| _ => false
+end.
+
 (* Do not check if their tailc flags match. Softbound changes the flag for
  * system calls, say atoi from tailcall to non-tailcall.
  *)
-Definition tv_scall fid (c1 c2:scall) :=
-  let '(stmn_call rid1 nr1 _ t1 v1 tsts1) := c1 in
-  let '(stmn_call rid2 nr2 _ t2 v2 tsts2) := c2 in
-  eq_id rid1 rid1 &&
-  (sumbool2bool _ _ (noret_dec nr1 nr2)) &&
-  tv_typ t1 t2 && tv_params fid tsts1 tsts2 &&
-  match (v1, v2) with
-  | (value_const (const_gid _ fid1), value_const (const_gid _ fid2)) => 
-      tv_fid fid1 fid2
-  | (v1, v2) => sumbool2bool _ _ (value_dec v1 v2)
+
+Inductive sicall : Set :=
+| stmn_icall_nptr : 
+    id -> noret -> tailc -> typ -> sterm -> list (typ*sterm) -> sicall
+| stmn_icall_ptr : 
+    id -> id -> id -> typ -> sterm -> sterm -> list (typ*sterm) -> sicall
+.
+
+Definition se_icall (st:sstate) (i:icall) : sicall :=
+match i with
+| icall_nptr id0 nr tc t0 v0 p0 =>
+    stmn_icall_nptr id0 nr tc t0 (value2Sterm st.(STerms) v0) 
+      (list_param__list_typ_subst_sterm p0 st.(STerms))
+| icall_ptr id0 id1 id2 t0 v0 id4 p0 =>
+    stmn_icall_ptr id0 id1 id2 t0 (value2Sterm st.(STerms) v0) 
+      (lookupSmap st.(STerms) id4)
+      (list_param__list_typ_subst_sterm p0 st.(STerms))
+end.
+
+Inductive scall : Set :=
+| stmn_call : id -> noret -> tailc -> typ -> sterm -> list (typ*sterm) -> scall
+.
+
+Definition se_call : forall (st : sstate)(i:cmd)(iscall:isCall i = true), scall.
+Proof.
+  intros. unfold isCall in iscall.
+  destruct i0; try solve [inversion iscall].
+  apply (@stmn_call i0 n t t0 (value2Sterm st.(STerms) v) 
+                      (list_param__list_typ_subst_sterm p st.(STerms))).
+Defined.
+
+Definition tv_scall Ps1 Ps2 fid (c1:scall) (c2:sicall) :=
+  let '(stmn_call rid1 nr1 _ ty1 t1 tsts1) := c1 in
+  match c2 with
+  | stmn_icall_nptr rid2 nr2 _ ty2 t2 tsts2 =>
+    tv_id fid rid1 rid2 &&
+    (sumbool2bool _ _ (noret_dec nr1 nr2)) &&
+    tv_typ ty1 ty2 && tv_params Ps1 Ps2 fid tsts1 tsts2 && 
+    tv_sterm Ps1 Ps2 fid (remove_cast t1) (remove_cast t2)
+  | stmn_icall_ptr rid2 _ _ ty2 t2 _ tsts2 =>
+    tv_id fid rid1 rid2 &&
+    tv_typ ty1 ty2 && tv_params Ps1 Ps2 fid tsts1 tsts2 && 
+    match (remove_cast t1, remove_cast t2) with
+    | (sterm_val (value_const (const_gid _ fid1)),
+       sterm_val (value_const (const_gid _ fid2))) =>
+      tv_fid fid1 fid2 && function_returns_pointer Ps1 fid2
+    | (st1, st2) => tv_sterm Ps1 Ps2 fid st1 st2
+    end
   end.
 
-Definition tv_subblock fid (sb1 sb2:subblock) :=
+Definition tv_subblock Ps1 Ps2 fid (sb1:subblock) (sb2:isubblock) :=
 match (sb1, sb2) with
-| (mkSB nbs1 call1 iscall1, mkSB nbs2 call2 iscall2) =>
+| (mkSB nbs1 call1 iscall1, mkiSB nbs2 call2) =>
   let st1 := se_cmds sstate_init nbs1 in
   let st2 := se_cmds sstate_init nbs2 in
   let cl1 := se_call st1 call1 iscall1 in
-  let cl2 := se_call st2 call2 iscall2 in
-   (sumbool2bool _ _ (sstate_sub_dec fid st1 st2 (se_cmds_init_uniq nbs1)))
+  let cl2 := se_icall st2 call2 in
+   (sumbool2bool _ _ 
+     (sstate_sub_dec Ps1 Ps2 fid st1 st2 (se_cmds_init_uniq nbs1))) &&
+   tv_scall Ps1 Ps2 fid cl1 cl2 
 end.
 
-Fixpoint tv_subblocks fid (sbs1 sbs2:list subblock) :=
+Fixpoint tv_subblocks Ps1 Ps2 fid (sbs1:list subblock) (sbs2:list isubblock) :=
 match (sbs1, sbs2) with
 | (nil, nil) => true
 | (sb1::sbs1', sb2::sbs2') => 
-    (tv_subblock fid sb1 sb2) && (tv_subblocks fid sbs1' sbs2')
+    (tv_subblock Ps1 Ps2 fid sb1 sb2) && (tv_subblocks Ps1 Ps2 fid sbs1' sbs2')
 | _ => false
 end.
 
@@ -804,10 +1126,82 @@ Fixpoint tv_phinodes fid (ps1 ps2:phinodes) : bool :=
 match ps1 with
 | nil => true
 | (insn_phi i1 _ _)as p1::ps1' =>
-  match lookupPhinode ps2 i1 with
+  match lookupPhinode ps2 (rename_id fid i1) with
   | None => false
   | Some p2 => tv_phinode fid p1 p2 && tv_phinodes fid ps1' ps2
   end
+end.
+
+(*
+  For a function that returns a pointer, Softbound translates
+         ret i32* %8                                                           
+  into
+         %.ptr = getelementptr { i32*, i8*, i8* }* %shadow_ret, i32 0, i32 0
+         %.base = getelementptr { i32*, i8*, i8* }* %shadow_ret, i32 0, i32 1
+         store i8* %bitcast, i8** %.base
+         %.bound = getelementptr { i32*, i8*, i8* }* %shadow_ret, i32 0, i32 2
+         store i8* %bitcast4, i8** %.bound
+         store i32* %8, i32** %.ptr
+         ret void
+ 
+  gen_iret returns %shadow_ret %.base %.base %.ptr i32* 
+*)
+Definition gen_iret t0 id0 (c1 c2 c3 c4 c5 c6:cmd) :=
+match c1 with
+|insn_gep id11 _ 
+(*
+   FIXME: This can also be a namedt...  We should formalize the type
+   equivalence algorithm.
+
+   (typ_struct 
+     (Cons_list_typ (typ_pointer _ as t01) 
+     (Cons_list_typ (typ_pointer _ as t02)
+     (Cons_list_typ (typ_pointer _ as t03) Nil_list_typ))) as t1)
+*)
+   t1
+   (value_id id12)
+   (Cons_list_value (value_const (const_int _ i11 as c11)) 
+     (Cons_list_value (value_const (const_int _ i12 as c12)) 
+      Nil_list_value)) =>
+  match c2 with 
+  |insn_gep id21 _ t2 (value_id id22) 
+     (Cons_list_value (value_const (const_int _ i21 as c21)) 
+       (Cons_list_value (value_const (const_int _ i22 as c22)) 
+       Nil_list_value)) =>
+    match c3 with
+    |insn_store id31 t3 v3 (value_id id32) _ =>
+      match c4 with
+      |insn_gep id41 _ t4 (value_id id42)
+         (Cons_list_value (value_const (const_int _ i41 as c41)) 
+         (Cons_list_value (value_const (const_int _ i42 as c42)) 
+            Nil_list_value)) =>
+        match c5 with
+        |insn_store id51 t5 v5 (value_id id52) _ =>
+           match c6 with
+           |insn_store id61 t6 v6 (value_id id62) _ =>
+              if (tv_typ t0 (typ_pointer t1) && tv_typ t1 t2 && tv_typ t2 t4 &&
+(*
+                  tv_typ t6 t01 && tv_typ t3 t02 && tv_typ t5 t03 &&
+                  tv_typ t02 t03 &&
+*)
+                  eq_id id0 id12 && eq_id id12 id22 && eq_id id22 id42 &&
+                  eq_id id11 id62 && eq_id id21 id32 && eq_id id41 id52 &&
+                  eq_const c11 c12 && eq_const c11 c21 && eq_const c11 c41
+                 ) 
+              then 
+                Some (id12, v3, v5, v6, t6)
+              else None
+           | _ => None
+           end
+        | _ => None
+        end
+      | _ => None
+      end
+    | _ => None
+    end
+  | _ => None
+  end
+| _ => None
 end.
 
 Definition tv_terminator fid (tmn1 tmn2:terminator) : bool :=
@@ -823,39 +1217,91 @@ match (tmn1, tmn2) with
 | _ => false
 end.
 
-Definition tv_block fid (b1 b2:block) :=
-match (b1, b2) with
-| (block_intro l1 ps1 cs1 tmn1, block_intro l2 ps2 cs2 tmn2) =>
-  match (cmds2sbs cs1, cmds2sbs cs2) with
-  | ((sbs1, nbs1), (sbs2, nbs2)) =>
-    eq_l l1 l2 && tv_phinodes fid ps1 ps2 && tv_subblocks fid sbs1 sbs2 &&
-    tv_cmds fid nbs1 nbs2 && tv_terminator fid tmn1 tmn2
-  end
+Definition get_last_six_insns (cs:cmds) :=
+match (List.rev cs) with
+| c6::c5::c4::c3::c2::c1::cs' => (List.rev cs', Some (c1, c2, c3, c4, c5, c6))
+| _ => (cs, None)
 end.
 
-Fixpoint tv_blocks fid (bs1 bs2:blocks):=
+Definition tv_block Ps1 Ps2 fid (b1 b2:block) :=
+match (b1, b2) with
+| (block_intro l1 ps1 cs1 tmn1, block_intro l2 ps2 cs2 tmn2) =>
+  let '(cs2', op) :=
+    match lookupFdefViaIDFromProducts Ps1 fid with      
+    | Some (fdef_intro (fheader_intro (typ_pointer _ as tp) _ _) _) =>
+      match lookupFdefViaIDFromProducts Ps2 (rename_fid fid) with 
+      | Some (fdef_intro (fheader_intro _ _ ((t2,id2)::_)) _) =>
+          let '(cs2', opcs6) := get_last_six_insns cs2 in
+          match opcs6 with
+          | Some (c1,c2,c3,c4,c5,c6) => 
+             (* gen_iret returns %shadow_ret %.base %.base %.ptr i32 *)
+             match gen_iret t2 id2 c1 c2 c3 c4 c5 c6 with
+             | None => (cs2, None)
+             | op => (cs2', op)
+             end
+          | None => (cs2, None)
+          end
+      | _ => (cs2, None)
+      end
+    | _ => (cs2, None)
+    end in 
+  match (cmds2sbs cs1, cmds2isbs Ps1 cs2') with
+  | ((sbs1, nbs1), (sbs2, nbs2)) =>
+    eq_l l1 l2 && tv_phinodes fid ps1 ps2 && 
+    tv_subblocks Ps1 Ps2 fid sbs1 sbs2 &&
+    tv_cmds Ps1 Ps2 fid nbs1 nbs2 && 
+    match op with 
+    | Some (id20, v21, v22, v23, t20) =>
+        match (tmn1, tmn2) with
+        | (insn_return id1 t1 v1, insn_return_void _) => tv_value fid v1 v23
+        | _ => tv_terminator fid tmn1 tmn2
+        end
+    | None => tv_terminator fid tmn1 tmn2
+    end
+  end 
+end.
+
+Fixpoint tv_blocks Ps1 Ps2 fid (bs1 bs2:blocks):=
 match (bs1, bs2) with
 | (nil, nil) => true
-| (b1::bs1', b2::bs2') => tv_block fid b1 b2 && tv_blocks fid bs1' bs2'
+| (b1::bs1', b2::bs2') => 
+    tv_block Ps1 Ps2 fid b1 b2 && tv_blocks Ps1 Ps2 fid bs1' bs2'
 | _ => false
 end.
 
-Definition tv_fheader (f1 f2:fheader) := 
+Definition tv_fheader Ps1 (f1 f2:fheader) := 
   let '(fheader_intro t1 fid1 a1) := f1 in
   let '(fheader_intro t2 fid2 a2) := f2 in
-  (sumbool2bool _ _ (typ_dec t1 t2)) &&
   tv_fid fid1 fid2 &&
-  (sumbool2bool _ _ (prefix_dec _ arg_dec a1 a2)).
+  if (function_returns_pointer Ps1 fid2) then
+    if (syscall_returns_pointer fid1) then true
+    else
+      match a2 with
+(*
+    | (typ_pointer (typ_struct 
+        (Cons_list_typ t21
+        (Cons_list_typ _
+        (Cons_list_typ _ Nil_list_typ)))),_)::a2' =>
+      (sumbool2bool _ _ (typ_dec t1 t21)) &&
+      (sumbool2bool _ _ (prefix_dec _ arg_dec a1 a2'))
+*)
+      | (typ_pointer _,_)::a2' =>
+        (sumbool2bool _ _ (prefix_dec _ arg_dec a1 a2'))
+      | _ => false
+      end
+  else
+    (sumbool2bool _ _ (typ_dec t1 t2)) &&
+    (sumbool2bool _ _ (prefix_dec _ arg_dec a1 a2)).
 
-Definition tv_fdec (f1 f2:fdec) :=
+Definition tv_fdec Ps1 (f1 f2:fdec) :=
 match (f1, f2) with
-| (fdec_intro fh1, fdec_intro fh2) => tv_fheader fh1 fh2
+| (fdec_intro fh1, fdec_intro fh2) => tv_fheader Ps1 fh1 fh2
 end.
 
-Definition tv_fdef (f1 f2:fdef) :=
+Definition tv_fdef Ps1 Ps2 (f1 f2:fdef) :=
 match (f1, f2) with
 | (fdef_intro (fheader_intro _ fid1 _ as fh1) lb1, fdef_intro fh2 lb2) =>
-  tv_fheader fh1 fh2 && tv_blocks fid1 lb1 lb2
+  tv_fheader Ps1 fh1 fh2 && tv_blocks Ps1 Ps2 fid1 lb1 lb2
 end.
 
 Fixpoint lookupGvarViaIDFromProducts (lp:products) (i:id) : option gvar :=
@@ -867,23 +1313,23 @@ match lp with
 | _::lp' => lookupGvarViaIDFromProducts lp' i
 end.
 
-Fixpoint tv_products (Ps1 Ps2:products) : bool :=
+Fixpoint tv_products (Ps10 Ps1 Ps2:products) : bool :=
 match Ps1 with
 | nil => true
 | product_gvar gv1::Ps1' =>
   match lookupGvarViaIDFromProducts Ps2 (getGvarID gv1) with
   | None => false
-  | Some gv2 => sumbool2bool _ _ (gvar_dec gv1 gv2) && tv_products Ps1' Ps2 
+  | Some gv2 => sumbool2bool _ _ (gvar_dec gv1 gv2) && tv_products Ps10 Ps1' Ps2 
   end
 | product_fdec f1::Ps1' =>
   match lookupFdecViaIDFromProducts Ps2 (rename_fid (getFdecID f1)) with
   | None => false
-  | Some f2 => tv_fdec f1 f2 && tv_products Ps1' Ps2 
+  | Some f2 => tv_fdec Ps10 f1 f2 && tv_products Ps10 Ps1' Ps2 
   end
 | product_fdef f1::Ps1' =>
   match lookupFdefViaIDFromProducts Ps2 (rename_fid (getFdefID f1)) with
   | None => false
-  | Some f2 => tv_fdef f1 f2 && tv_products Ps1' Ps2 
+  | Some f2 => tv_fdef Ps10 Ps2 f1 f2 && tv_products Ps10 Ps1' Ps2 
   end
 end.
 
@@ -892,7 +1338,7 @@ match (m1, m2) with
 | (module_intro los1 nts1 Ps1, module_intro los2 nts2 Ps2) =>
   sumbool2bool _ _ (layouts_dec los1 los2) &&
   sumbool2bool _ _ (namedts_dec nts1 nts2) &&
-  tv_products Ps1 Ps2
+  tv_products Ps1 Ps1 Ps2
 end.
 
 Fixpoint tv_system (S1 S2:system) :=
@@ -1104,7 +1550,7 @@ match sm with
   else safe_mem_access fid sm1 t ptr
 end.
 
-Fixpoint sterm_is_memsafe fid l (st:sterm) : bool :=
+Fixpoint sterm_is_memsafe Ps1 Ps2 fid l (st:sterm) : bool :=
 match st with
 | sterm_val v => true
 | sterm_bop _ _ st1 st2 
@@ -1112,54 +1558,59 @@ match st with
 | sterm_icmp _ _ st1 st2 
 | sterm_fcmp _ _ st1 st2 
 | sterm_insertvalue _ st1 _ st2 _ => 
-    sterm_is_memsafe fid l st1 && sterm_is_memsafe fid l st2 
+    sterm_is_memsafe Ps1 Ps2 fid l st1 && sterm_is_memsafe Ps1 Ps2 fid l st2 
 | sterm_trunc _ _ st1 _
 | sterm_ext _ _ st1 _ 
 | sterm_cast _ _ st1 _ 
-| sterm_extractvalue _ st1 _ => sterm_is_memsafe fid l st1
+| sterm_extractvalue _ st1 _ => sterm_is_memsafe Ps1 Ps2 fid l st1
 | sterm_malloc sm _ st1 _
 | sterm_alloca sm _ st1 _ => 
-    smem_is_memsafe fid l sm && sterm_is_memsafe fid l st1
+    smem_is_memsafe Ps1 Ps2 fid l sm && sterm_is_memsafe Ps1 Ps2 fid l st1
 | sterm_load sm t st1 _ => 
-   smem_is_memsafe fid l sm && sterm_is_memsafe fid l st1 && 
+   smem_is_memsafe Ps1 Ps2 fid l sm && sterm_is_memsafe Ps1 Ps2 fid l st1 && 
    safe_mem_access fid sm t st1
 | sterm_gep _ _ st1 sts2 => 
-   sterm_is_memsafe fid l st1 && list_sterm_is_memsafe fid l sts2
-| sterm_phi _ stls => list_sterm_l_is_memsafe fid l stls
+   sterm_is_memsafe Ps1 Ps2 fid l st1 && list_sterm_is_memsafe Ps1 Ps2 fid l sts2
+| sterm_phi _ stls => list_sterm_l_is_memsafe Ps1 Ps2 fid l stls
 | sterm_select st1 _ st2 st3 => 
-    sterm_is_memsafe fid l st1 && sterm_is_memsafe fid l st2 && 
-    sterm_is_memsafe fid l st3
+    sterm_is_memsafe Ps1 Ps2 fid l st1 && sterm_is_memsafe Ps1 Ps2 fid l st2 && 
+    sterm_is_memsafe Ps1 Ps2 fid l st3
 | sterm_lib sm lid sts => 
-    smem_is_memsafe fid l sm && list_sterm_is_memsafe fid l sts && 
+    smem_is_memsafe Ps1 Ps2 fid l sm && 
+    list_sterm_is_memsafe Ps1 Ps2 fid l sts && 
     store_to_metadata fid l sm lid sts
 end
-with list_sterm_is_memsafe fid l (sts:list_sterm) : bool :=
+with list_sterm_is_memsafe Ps1 Ps2 fid l (sts:list_sterm) : bool :=
 match sts with
 | Nil_list_sterm => true
 | Cons_list_sterm st sts0 => 
-    sterm_is_memsafe fid l st && list_sterm_is_memsafe fid l sts0
+    sterm_is_memsafe Ps1 Ps2 fid l st && list_sterm_is_memsafe Ps1 Ps2 fid l sts0
 end
-with list_sterm_l_is_memsafe fid l (stls:list_sterm_l) : bool :=
+with list_sterm_l_is_memsafe Ps1 Ps2 fid l (stls:list_sterm_l) : bool :=
 match stls with
 | Nil_list_sterm_l => true
 | Cons_list_sterm_l st _ stls0 =>
-    sterm_is_memsafe fid l st && list_sterm_l_is_memsafe fid l stls0
+    sterm_is_memsafe Ps1 Ps2 fid l st && 
+    list_sterm_l_is_memsafe Ps1 Ps2 fid l stls0
 end
-with smem_is_memsafe fid l (sm:smem) : bool :=
+with smem_is_memsafe Ps1 Ps2 fid l (sm:smem) : bool :=
 match sm with
 | smem_init => true
 | smem_malloc sm1 _ st1 _
 | smem_alloca sm1 _ st1 _ => 
-    smem_is_memsafe fid l sm1 && sterm_is_memsafe fid l st1
+    smem_is_memsafe Ps1 Ps2 fid l sm1 && sterm_is_memsafe Ps1 Ps2 fid l st1
 | smem_free sm1 _ _ => false
 | smem_load sm1 t st1 _ => 
-    smem_is_memsafe fid l sm1 && sterm_is_memsafe fid l st1 && 
+    smem_is_memsafe Ps1 Ps2 fid l sm1 && sterm_is_memsafe Ps1 Ps2 fid l st1 && 
     safe_mem_access fid sm1 t st1
 | smem_store sm1 t st11 st12 _ =>
-    smem_is_memsafe fid l sm1 && sterm_is_memsafe fid l st11 && 
-    sterm_is_memsafe fid l st12 && safe_mem_access fid sm1 (typ_pointer t) st12
+    smem_is_memsafe Ps1 Ps2 fid l sm1 && sterm_is_memsafe Ps1 Ps2 fid l st11 && 
+    sterm_is_memsafe Ps1 Ps2 fid l st12 && 
+    (store_to_ret Ps1 Ps2 fid st12 || 
+     safe_mem_access fid sm1 (typ_pointer t) st12)
 | smem_lib sm1 lid1 sts1 =>
-    smem_is_memsafe fid l sm1 && list_sterm_is_memsafe fid l sts1 && 
+    smem_is_memsafe Ps1 Ps2 fid l sm1 && 
+    list_sterm_is_memsafe Ps1 Ps2 fid l sts1 && 
     deref_check fid l lid1 sts1
 end.
 
@@ -1202,9 +1653,9 @@ end.
 Definition check_addrof_be fid sm :=
   check_addrof_be_aux fid sm (get_addrof_be tt).
 
-Definition mtv_cmds fid l (nbs2 : list nbranch) :=
+Definition mtv_cmds Ps1 Ps2 fid l (nbs2 : list nbranch) :=
 let st2 := se_cmds sstate_init nbs2 in 
-smem_is_memsafe fid l st2.(SMem) &&
+smem_is_memsafe Ps1 Ps2 fid l st2.(SMem) &&
 check_all_metadata fid l st2.(STerms) &&
 check_addrof_be fid st2.(STerms).
 
@@ -1242,10 +1693,11 @@ end.
     l1:
       call fid2 tsts2   
 *)
-Definition mtv_scall Ps2 fid l1 (c2:scall) :=
-  let '(stmn_call _ _ _ _ v2 tsts2) := c2 in
-  match v2 with
-  | value_const (const_gid _ fid2) =>
+Definition mtv_iscall Ps2 fid l1 (c2:sicall) :=
+match c2 with
+| stmn_icall_nptr _ _ _ _ t2 tsts2 =>
+  match t2 with
+  | sterm_val (value_const (const_gid _ fid2)) =>
       if (isCallLib fid2) then true
       else
         match (lookupFdefViaIDFromProducts Ps2 fid2) with
@@ -1254,23 +1706,37 @@ Definition mtv_scall Ps2 fid l1 (c2:scall) :=
             mtv_func_metadata (get_metadata tt) fid l1 fid2 args2 tsts2
         end
   | _ => true
-  end.
-
-Definition mtv_subblock Ps2 fid l (sb2:subblock) :=
-match sb2 with
-| mkSB nbs2 call2 iscall2 =>
-  let st2 := se_cmds sstate_init nbs2 in
-  let cl2 := se_call st2 call2 iscall2 in
-   smem_is_memsafe fid l st2.(SMem) &&
-   check_all_metadata fid l st2.(STerms) &&
-   check_addrof_be fid st2.(STerms) &&
-   mtv_scall Ps2 fid l cl2
+  end
+| stmn_icall_ptr _ _ _ _ t2 _ tsts2 =>
+  match t2 with
+  | sterm_val (value_const (const_gid _ fid2)) =>
+      if (isCallLib fid2) then true
+      else
+        match (lookupFdefViaIDFromProducts Ps2 fid2) with
+        | None => true
+        | Some (fdef_intro (fheader_intro _ _ args2) _) =>
+            mtv_func_metadata (get_metadata tt) fid l1 fid2 args2 tsts2
+        end
+  | _ => true
+  end
 end.
 
-Fixpoint mtv_subblocks Ps2 fid l (sbs2:list subblock) :=
+Definition mtv_isubblock Ps1 Ps2 fid l (sb2:isubblock) :=
+match sb2 with
+| mkiSB nbs2 call2 =>
+  let st2 := se_cmds sstate_init nbs2 in
+  let cl2 := se_icall st2 call2 in
+   smem_is_memsafe Ps1 Ps2 fid l st2.(SMem) &&
+   check_all_metadata fid l st2.(STerms) &&
+   check_addrof_be fid st2.(STerms) &&
+   mtv_iscall Ps2 fid l cl2
+end.
+
+Fixpoint mtv_isubblocks Ps1 Ps2 fid l (sbs2:list isubblock) :=
 match sbs2 with
 | nil => true
-| sb2::sbs2' => mtv_subblock Ps2 fid l sb2 && mtv_subblocks Ps2 fid l sbs2'
+| sb2::sbs2' => 
+    mtv_isubblock Ps1 Ps2 fid l sb2 && mtv_isubblocks Ps1 Ps2 fid l sbs2'
 end.
 
 (* Check
@@ -1322,38 +1788,38 @@ end.
 Definition mtv_phinodes fid l (ps2:phinodes) : bool :=
   mtv_phinodes_aux fid l (get_metadata tt) ps2.
 
-Definition mtv_block Ps2 fid (b2:block) :=
+Definition mtv_block Ps1 Ps2 fid (b2:block) :=
 match b2 with
 | block_intro l2 ps2 cs2 tmn2 =>
   mtv_phinodes fid l2 ps2 &&
-  match cmds2sbs cs2 with
+  match cmds2isbs Ps1 cs2 with
   | (sbs2, nbs2) =>
-    mtv_subblocks Ps2 fid l2 sbs2 && mtv_cmds fid l2 nbs2
+    mtv_isubblocks Ps1 Ps2 fid l2 sbs2 && mtv_cmds Ps1 Ps2 fid l2 nbs2
   end
 end.
 
-Fixpoint mtv_blocks Ps2 fid (bs2:blocks):=
+Fixpoint mtv_blocks Ps1 Ps2 fid (bs2:blocks):=
 match bs2 with
 | nil => true
-| b2::bs2' => mtv_block Ps2 fid b2 && mtv_blocks Ps2 fid bs2'
+| b2::bs2' => mtv_block Ps1 Ps2 fid b2 && mtv_blocks Ps1 Ps2 fid bs2'
 end.
 
-Definition mtv_fdef Ps2 (f2:fdef) :=
+Definition mtv_fdef Ps1 Ps2 (f2:fdef) :=
 match f2 with
 | fdef_intro ((fheader_intro t2 fid2 a2) as fh2) lb2 =>
-  if (isCallLib fid2) then true else mtv_blocks Ps2 fid2 lb2
+  if (isCallLib fid2) then true else mtv_blocks Ps1 Ps2 fid2 lb2
 end.
 
-Fixpoint mtv_products (Ps Ps2:products) : bool :=
+Fixpoint mtv_products Ps1 (Ps20 Ps2:products) : bool :=
 match Ps2 with
 | nil => true
-| product_fdef f2::Ps2' => mtv_fdef Ps f2 && mtv_products Ps Ps2'
-| _::Ps2' => mtv_products Ps Ps2'
+| product_fdef f2::Ps2' => mtv_fdef Ps1 Ps20 f2 && mtv_products Ps1 Ps20 Ps2'
+| _::Ps2' => mtv_products Ps1 Ps20 Ps2'
 end.
 
-Definition mtv_module (m2:module) :=
-match m2 with
-| module_intro los2 nts2 Ps2 => mtv_products Ps2 Ps2
+Definition mtv_module (m1:module) (m2:module) :=
+match (m1, m2) with
+| (module_intro _ _ Ps1, module_intro _ _ Ps2) => mtv_products Ps1 Ps2 Ps2
 end.
 
 (***********************************)
